src/named/Decidable.v
@@ -1,0 +1,335 @@
+Require Import mathcomp.ssreflect.all_ssreflect.
+Set Implicit Arguments.
+Unset Strict Implicit.
+Unset Printing Implicit Defensive.
+Set Bullet Behavior "Strict Subproofs".
+
+
+From Ltac2 Require Import Ltac2.
+From Utils Require Import Utils.
+From Named Require Import Exp Rule ARule Tactics.
+From Named Require ICore.
+Import ICore.IndependentJudgment.
+Import Exp.Notations ARule.Notations. (* TODO: Rule.Notations.*)
+Require Import String.
+
+Require Import Named.Recognizers.
+
+Set Default Proof Mode "Ltac2".
+
+
+(*TODO: weaken to recognize for now? eventually want reflect?*)
+Class LangRecognize (l : lang) : Type :=
+  {
+  le_sort_dec : nat -> ctx -> sort -> sort -> bool;
+  decide_le_sort : forall n c t1 t2,
+      wf_lang (nth_tail n l) ->
+      wf_sort (nth_tail n l) c t1 ->
+      wf_sort (nth_tail n l) c t2 ->
+      (le_sort_dec n c t1 t2) -> (le_sort (nth_tail n l) c t1 t2);
+  term_args_elab : ctx -> list exp -> string -> sort -> list exp;
+  (* only needed for proof of other direction *)
+  (*elaborate_term_implicits
+  : forall n c name s t,
+      let r := named_list_lookup (sort_rule [::] [::]) l name in
+      let args := get_rule_args r in
+      let c' := get_rule_ctx r in
+      let t' := get_rule_sort r in
+      wf_lang (nth_tail n l) ->
+      (wf_term (nth_tail n l) c (con name s) t)
+      <-> wf_args (nth_tail n l) c s args (term_args_elab c s name t) c';*)
+  sort_args_elab : ctx -> list exp -> string -> list exp;
+  (*elaborate_sort_implicits
+  : forall n c name s,
+      let r := named_list_lookup (sort_rule [::] [::]) l name in
+      let args := get_rule_args r in
+      let c' := get_rule_ctx r in
+      wf_lang (nth_tail n l) ->
+      (wf_sort (nth_tail n l) c (scon name s))
+      <-> wf_args (nth_tail n l) c s args (sort_args_elab c s name) c'*)
+  }.
+
+Section Base.
+
+  Variable l : lang.
+  Context (langrec : LangRecognize l).
+
+
+  (* TODO: not well-founded b/c of implicit arguments! need a rule about implicits depth.
+     For now I will only reason about recognization.
+   *)
+  (*Parameter implicits_size_cap : nat.
+  
+  
+
+  Fixpoint depth (e : exp) : nat :=
+    match e with
+    | con _ s => (foldr max 0 (map depth s)).+2
+    | var _ => 0
+    end.
+  Definition args_depth s : nat := (foldr max 0 (map depth s)).+1.
+   *)     
+  
+  Fixpoint wf_term_dec n c e t fuel : bool :=
+    match fuel, e with
+    | 0,_ => false
+    | S fuel', var x =>
+      match named_list_lookup_err c x with
+      | Some t' => le_sort_dec n c t' t
+      | None => false
+      end
+    | S fuel', con name s =>
+      match named_list_lookup_err (nth_tail n l) name with
+      | Some (term_rule c' args t') =>
+        let es := term_args_elab c s name t in
+        (wf_sort_dec n c t'[/with_names_from c' es/] fuel') &&
+        (le_sort_dec n c t'[/with_names_from c' es/] t) &&
+        (wf_args_dec n c s args es c' fuel')
+      | _ => false
+      end
+    end
+  with wf_args_dec n c s args es c' fuel : bool :=
+         match fuel, c',es, args, s with
+         | 0,_,_,_,_=> false
+         | S fuel', [::], [::], [::], [::] => true
+         | S fuel', [::], _, _, _ => false
+         | S fuel', (name,t)::c'', [::], _, _ => false
+         | S fuel', (name,t)::c'', e::es', [::], [::] =>
+           (wf_term_dec n c e t[/with_names_from c'' es'/] fuel') &&
+           (wf_args_dec n c [::] [::] es' c'' fuel')
+         | S fuel', (name,t)::c'', e::es', name'::args', e'::s' =>
+           if name == name'
+           then (e == e') &&
+                (wf_term_dec n c e t[/with_names_from c'' es'/] fuel') &&
+                (wf_args_dec n c s' args' es' c'' fuel')
+           else (wf_term_dec n c e t[/with_names_from c'' es'/] fuel') &&
+                (wf_args_dec n c s args es' c'' fuel')
+         | _,_,_,_,_ => false (*TODO*)
+         end
+  with wf_sort_dec n c t fuel : bool :=
+    match fuel, t with
+    | 0,_ => false
+    | S fuel', scon name s =>
+      match named_list_lookup_err (nth_tail n l) name with
+      | Some (sort_rule c' args) =>
+        let es := sort_args_elab c s name in
+        (wf_args_dec n c s args es c' fuel')
+      | _ => false
+      end
+    end.
+
+  Arguments wf_term_dec n c !e t !fuel/.
+  Arguments wf_args_dec n c !s !args !es !c' !fuel/.
+  Arguments wf_sort_dec n c !t !fuel/.
+
+  Lemma decide_wf_term n c e t fuel
+    : wf_lang (nth_tail n l) ->
+      wf_ctx (nth_tail n l) c ->
+      wf_sort (nth_tail n l) c t ->
+      wf_term_dec n c e t fuel -> wf_term (nth_tail n l) c e t
+  with decide_wf_args n c s args es c' fuel
+       : wf_lang (nth_tail n l) ->
+         wf_ctx (nth_tail n l) c ->
+         wf_ctx (nth_tail n l) c' ->
+         wf_args_dec n c s args es c' fuel -> wf_args (nth_tail n l) c s args es c'
+  with decide_wf_sort n c t fuel
+       : wf_lang (nth_tail n l) ->
+         wf_ctx (nth_tail n l) c ->
+         wf_sort_dec n c t fuel -> wf_sort (nth_tail n l) c t.
+  Proof using Type.
+    {
+      intros wfl wfc wfs.
+      destruct fuel> [intro fls; inversion fls|].
+      destruct e; simpl;
+        repeat (ltac1:(case_match)); try (solve[intro fls; inversion fls]).
+      {
+        intros.
+        eapply wf_term_conv>[| |apply decide_le_sort in H; eauto].
+        admit.
+        constructor.
+        ltac1:(simple apply (@named_list_lookup_err_in)).
+        symmetry; eauto.
+        admit.
+      }
+      {
+        repeat ltac1:(move => /andP []).
+        intros.        
+        eapply wf_term_conv>[| |apply decide_le_sort in b; eauto]; auto.
+        (*wf sort subst*)admit.
+        eapply wf_term_by; simpl; auto.
+        ltac1:(simple apply (@named_list_lookup_err_in)).
+        symmetry; eauto.
+        apply decide_wf_args in b0; auto.
+        (* wf_rule in *)admit.
+      }
+    }
+    {
+      intros wfl wfc wfc'.
+      destruct fuel> [intro fls; inversion fls|].
+      destruct c'; destruct es; ltac1:(break);
+        destruct args; destruct s; ltac1:(break);simpl;
+          try (solve[intro fls; inversion fls]).
+      { constructor. }
+      {        
+        ltac1:(move => /andP []).
+        inversion wfc'; subst.
+        constructor; eauto.
+        eapply decide_wf_term; eauto.
+        (* sort subst pres. wf*) admit.
+      }
+      {
+        remember (s0==s2) as eqs; destruct eqs.
+        {
+          symmetry in Heqeqs.
+          ltac1:(move: Heqeqs => /eqP ?); subst.
+          inversion wfc'; subst.
+          repeat ltac1:(move => /andP []).
+          ltac1:(move => /eqP ?); subst.
+          constructor; eauto.
+          apply decide_wf_term in b; eauto.
+          (* sort subst pres. wf*) admit.
+        }
+        {
+          inversion wfc'; subst.
+          repeat ltac1:(move => /andP []).
+          intros.
+          apply wf_args_cons_im; eauto.
+          apply decide_wf_term in a; eauto.
+          (* sort subst pres. wf*) admit.
+        }
+      }
+    }
+    {
+      intros wfl wfc.
+      destruct fuel> [intro fls; inversion fls|].
+      destruct t; simpl;
+        repeat (ltac1:(case_match)); try (solve[intro fls; inversion fls]).
+      repeat ltac1:(move => /andP []).
+      ltac1:(move => /decide_wf_args wfa).
+      eapply wf_sort_by; simpl; auto.
+      ltac1:(simple apply (@named_list_lookup_err_in)).
+      symmetry; eauto.
+      apply wfa; auto.
+      (* from wf lang *)admit.
+    }
+  Admitted.
+
+  Fixpoint wf_ctx_dec n c fuel : bool :=
+    match c with
+    | [::] => true
+    | (name,t)::c'=>
+      (fresh name c') &&
+      (wf_sort_dec n c' t fuel) &&
+      (wf_ctx_dec n c' fuel)
+    end.
+
+  Arguments wf_ctx_dec n !c fuel/.
+
+  Lemma decide_wf_ctx n c fuel
+       : wf_lang (nth_tail n l) ->
+         wf_ctx_dec n c fuel -> wf_ctx (nth_tail n l) c.
+  Proof.
+    induction c; intros; ltac1:(break); simpl in *; constructor; auto;
+    revert H0;
+    repeat ltac1:(move => /andP []);
+    intros; auto.
+    eapply decide_wf_sort; eauto.
+  Qed.    
+
+  Definition wf_rule_dec n r fuel : bool :=
+    match r with
+    | sort_rule c args =>
+      (subseq args (map fst c)) &&
+      (wf_ctx_dec n c fuel)
+    | term_rule c args t =>
+      (subseq args (map fst c)) &&
+      (wf_ctx_dec n c fuel) &&
+      (wf_sort_dec n c t fuel)
+    | sort_le c t1 t2 =>
+      (wf_ctx_dec n c fuel) &&
+      (wf_sort_dec n c t1 fuel) &&
+      (wf_sort_dec n c t2 fuel)
+    | term_le c e1 e2 t =>
+      (wf_ctx_dec n c fuel) &&
+      (wf_term_dec n c e1 t fuel) &&
+      (wf_term_dec n c e2 t fuel) &&
+      (wf_sort_dec n c t fuel)
+    end.
+
+  Lemma decide_wf_rule n r fuel
+       : wf_lang (nth_tail n l) ->
+         wf_rule_dec n r fuel -> wf_rule (nth_tail n l) r.
+  Proof.
+    intro.
+    destruct r;
+    repeat ltac1:(move => /andP []);
+    intros; constructor; eauto using decide_wf_ctx, decide_wf_sort, decide_wf_term.
+  Qed.
+
+  Fixpoint wf_lang_dec' n l fuel : bool :=
+    match l with
+    | [::] => true
+    | (name,r)::l' =>
+      (fresh name l') &&
+      (wf_rule_dec n.+1 r fuel) &&
+      (wf_lang_dec' n.+1 l' fuel)
+    end.
+
+  Definition wf_lang_dec fuel : bool :=
+    wf_lang_dec' 0 l fuel.
+
+(*
+Lemma decide_wf_lang_succ n name r fuel
+  : wf_lang_dec' n.+1 (nth_tail n.+1 l) fuel ->
+    fresh name (nth_tail n.+1 l) ->
+    wf_rule_dec n r fuel ->
+    wf_lang_dec' n (nth_tail n l) fuel.
+Proof.
+  intros.
+  destruct l.
+  { destruct n; simpl; auto. }
+  {
+    destruct n; simpl; ltac1:(break); auto.
+    {
+      ltac1:(break_goal); auto.
+      unfold nth_tail in H.
+      repeat ltac1:(move => /andP []).      
+    simpl.
+  *)
+
+  Lemma decide_wf_lang' n fuel
+    : wf_lang_dec' n (nth_tail n l) fuel -> wf_lang (nth_tail n l).
+  Proof.
+    remember (nth_tail n l) as nl.
+    revert n Heqnl.
+    induction nl.
+    { constructor. }
+    {
+      intros; ltac1:(break); simpl in *.
+      revert H;
+        repeat ltac1:(move => /andP []);
+        intros.
+      constructor; auto.
+      {
+        eapply (IHnl (S n)).
+        ltac1:(simple eapply nth_tail_cons_eq); eauto.
+        assumption.
+      }
+      {
+        ltac1:(simple apply nth_tail_cons_eq in Heqnl).
+        rewrite Heqnl.
+        eapply decide_wf_rule; eauto.
+        rewrite <-Heqnl.
+        eauto.
+      }
+    }
+  Qed.
+
+  Lemma decide_wf_lang fuel : wf_lang_dec fuel -> wf_lang l.
+  Proof.
+    unfold wf_lang_dec.
+    apply decide_wf_lang'.
+  Qed.
+
+
+End Base.
