README.md
@@ -1,6 +1,15 @@
 #TODOs
 
-* Improve automation to be consistent across all uses (currently 3 versions)
+* restructure/rename file layout
+  + remove named/ hierarchy level
+  + clear old files in other dirs
+  + move IndependentJudgment out of ICore
+  + rename/expand or at least roadmap Decidable
+* Fully switch to independent judgment (no elab) for all existing languages
+* Relate independent judgment to original via elab to port theorems (or is it easier to replicate them?)
+* Clear admits in Decidable
+* Extend Decidable to work for compilers when possible
+* Improve automation to be consistent across all uses
 * determine whether there is an issue w/ current lax typing on le judgments
 * Either: remove IExp and use Exp for everything
 * Or: implement equality? and fill admits in subst lemmas for IExp
